Tap

Refinery/Term/Extrinsic/Wf/DerivedRewrite.lean
@@ -1,5 +1,6 @@
 import Refinery.Term.Extrinsic.Wf.Rewrite
 import Refinery.Term.Extrinsic.Wf.PreBeta
+import Refinery.Term.Extrinsic.Wf.WkEffect
 
 open HasQuant HasPQuant HasCommRel
 
@@ -10,7 +11,34 @@ namespace Term
 variable  {φ : Type u} {α : Type v} {ε : Type w} [S : Signature φ α ε]
           {R : DRWS φ α} [R.UWkCongr]
 
-def Eqv.let₂_let₂ {Γ Γl Γc Γm Γr : Ctx? α} {A B C D E}
+theorem Eqv.let₂_let₁ {Γ Γl Γc Γm Γr : Ctx? α} {A B C D}
+    (hΓ : Γ.SSplit Γl Γc) (hΓc : Γc.SSplit Γm Γr)
+    (a : Eqv R Γr A)
+    (b : Eqv R (Γm.cons ⟨A, ⊤⟩) (B.tensor C))
+    (c : Eqv R ((Γl.cons ⟨B, ⊤⟩).cons ⟨C, ⊤⟩) D)
+    : (a.let₁ hΓc b).let₂ hΓ c
+    = a.let₁ (hΓ.s1_23_12_3 hΓc) (b.let₂ (((hΓ.s1_23_12 hΓc).cons (.right _))) (c.wk2 _)) := by
+  rw [bind_let₂, let_let₁]
+  congr 1
+  conv => rhs; rw [bind_let₂]
+  congr 1
+  induction c using quotInd
+  apply sound; apply Wf.eqv.of_tm
+  simp [Wf.wk1, Wf.let₂, Wf.let₁, Wf.wk2, Wf.bv0, ren_ren, <-Nat.liftWk_comp, Nat.liftWk_comp_succ]
+
+theorem Eqv.let₂_let₁_anti {Γ Γl Γc Γm Γr : Ctx? α} {A B C D}
+    (hΓ : Γ.SSplit Γc Γr) (hΓc : Γc.SSplit Γl Γm)
+    (a : Eqv R Γr A)
+    (b : Eqv R (Γm.cons ⟨A, ⊤⟩) (B.tensor C))
+    (c : Eqv R ((Γl.cons ⟨B, ⊤⟩).cons ⟨C, ⊤⟩) D)
+    : a.let₁ hΓ (b.let₂ ((hΓc.cons (.right _))) (c.wk2 _))
+    = (a.let₁ (hΓ.s12_3_23 hΓc) b).let₂ (hΓ.s12_3_1_23 hΓc) c := by
+  rw [let₂_let₁]
+  induction a, b, c using quotInd₃
+  apply sound; apply Wf.eqv.of_tm
+  rfl
+
+theorem Eqv.let₂_let₂ {Γ Γl Γc Γm Γr : Ctx? α} {A B C D E}
     (hΓ : Γ.SSplit Γl Γc) (hΓc : Γc.SSplit Γm Γr)
     (a : Eqv R Γr (A.tensor B))
     (b : Eqv R ((Γm.cons ⟨A, ⊤⟩).cons ⟨B, ⊤⟩) (C.tensor D))
@@ -18,14 +46,26 @@ def Eqv.let₂_let₂ {Γ Γl Γc Γm Γr : Ctx? α} {A B C D E}
     : (a.let₂ hΓc b).let₂ hΓ c
     = a.let₂ (hΓ.s1_23_12_3 hΓc)
       (b.let₂ (((hΓ.s1_23_12 hΓc).cons (.right _)).cons (.right _)) ((c.wk2 _).wk2 _)) := by
-    rw [bind_let₂, let_let₂]
-    congr 1
-    conv => rhs; rw [bind_let₂]
-    congr 1
-    induction c using quotInd
-    apply sound; apply Wf.eqv.of_tm
-    simp [Wf.wk1, Wf.let₂, Wf.wk2, Wf.bv0, ren_ren, <-Nat.liftWk_comp, Nat.liftWk_comp_succ]
-    rfl
+  rw [bind_let₂, let_let₂]
+  congr 1
+  conv => rhs; rw [bind_let₂]
+  congr 1
+  induction c using quotInd
+  apply sound; apply Wf.eqv.of_tm
+  simp [Wf.wk1, Wf.let₂, Wf.wk2, Wf.bv0, ren_ren, <-Nat.liftWk_comp, Nat.liftWk_comp_succ]
+  rfl
+
+theorem Eqv.let₂_let₂_anti {Γ Γl Γc Γm Γr : Ctx? α} {A B C D E}
+    (hΓ : Γ.SSplit Γc Γr) (hΓc : Γc.SSplit Γl Γm)
+    (a : Eqv R Γr (A.tensor B))
+    (b : Eqv R ((Γm.cons ⟨A, ⊤⟩).cons ⟨B, ⊤⟩) (C.tensor D))
+    (c : Eqv R ((Γl.cons ⟨C, ⊤⟩).cons ⟨D, ⊤⟩) E)
+    : a.let₂ hΓ (b.let₂ ((hΓc.cons (.right _)).cons (.right _)) ((c.wk2 _).wk2 _))
+    = (a.let₂ (hΓ.s12_3_23 hΓc) b).let₂ (hΓ.s12_3_1_23 hΓc) c := by
+  rw [let₂_let₂]
+  induction a, b, c using quotInd₃
+  apply sound; apply Wf.eqv.of_tm
+  rfl
 
 theorem Eqv.bind_pair {Γ Γl Γr : Ctx? α}
     (hΓ : Γ.SSplit Γl Γr) (a : Eqv R Γl A) (b : Eqv R Γr B)
@@ -50,9 +90,176 @@ theorem Eqv.bind_pair_anti' {Γ Γl Γr Γe : Ctx? α} [hΓe : Γe.del]
   conv => rhs; rw [bind_pair]
   induction a, b using quotInd₂; apply sound; apply Wf.eqv.of_tm; rfl
 
-theorem Eqv.bind_pair_anti {Γ Γl Γr : Ctx? α}
+theorem Eqv.bind_pair_anti {A B} {Γ Γl Γr : Ctx? α}
     (hΓ : Γ.SSplit Γl Γr) (a : Eqv R Γr A) (b : Eqv R Γl B)
   : .let₁ hΓ a (.let₁ (Γl.erase_left.cons (.left _)) (b.wk0 _)
     (.pair (((Ctx?.both _).cons (.left _)).cons (.right _)) .bv1 .bv0))
     = a.pair hΓ.comm b
   := by rw [a.bind_pair_anti' hΓ]
+
+theorem Eqv.bind_pair_left {Γ Γl Γr : Ctx? α}
+    (hΓ : Γ.SSplit Γl Γr) (a : Eqv R Γl A) (b : Eqv R Γr B)
+  : a.pair hΓ b = .let₁ hΓ.comm a (.pair (Γr.erase_left.cons (.left _)) .bv0 (b.wk0 ⟨A, 0⟩))
+  := by
+  rw [bind_pair]
+  congr 1
+  induction b using quotInd with
+  | h b =>
+  apply sound
+  apply Wf.eqv.coh
+  exact Wf.pre_beta_pureLout (Γr.erase_left.cons (.left _))
+    (b.wk0 ⟨A, 0⟩)
+    (.pair ((Γr.erase.erase_left.cons (.left _)).cons (.right _)) .bv1 .bv0)
+  rfl
+  rfl
+
+--TODO: bind_pair_right_fwd
+
+--TODO: bind_pair_right_bwd
+
+theorem Eqv.bind_pair_right {A }{Γ Γl Γr : Ctx? α}
+  (hΓ : Γ.SSplit Γl Γr) (ea eb : ε)
+  (a : Eqv R Γl A) (b : Eqv R Γr B)
+  [ha : a.HasEff ea] [hb : b.HasEff eb] (he : ea ⇌ eb)
+  : a.pair hΓ b
+  = b.let₁ hΓ ((a.wk0 ⟨B, 0⟩).pair ((Γl.erase_right).cons (.right _)) .bv0)
+  := by
+  apply Eq.symm
+  cases ha; induction hb
+  rename_i ea a ha eb b hb
+  apply sound
+  apply Wf.eqv.coh
+  exact Wf.pre_beta hΓ b 1 (by simp)
+    (.pair ((Γl.erase_right).cons (.right _)) (a.wk0 ⟨B, 0⟩) .bv0)
+    (hb := inferInstance) he.symm (by generalize pquant ea = p; cases p; constructor <;> simp)
+  rfl
+  simp only [Wf.subst, Wf.wk0, Wf.bv0, Wf.pair, subst, SubstDS.subst0_get_zero, pair.injEq,
+    and_true]
+  rw [<-Term.subst_renIn]
+  apply Subst.subst1_fvi
+  intro x hx
+  simp [SubstDS.refl_get, lt_of_lt_of_le hx a.deriv.fvi_le_length]
+
+--TODO: bind_pair_comm_fwd
+
+--TODO: bind_pair_comm_bwd
+
+theorem Eqv.bind_pair_comm {A} {Γ Γl Γr : Ctx? α}
+  (hΓ : Γ.SSplit Γl Γr) {ea eb : ε}
+  (a : Eqv R Γl A) (b : Eqv R Γr B)
+  [ha : a.HasEff ea] [hb : b.HasEff eb] (he : ea ⇌ eb)
+  : a.pair hΓ b
+  = b.let₁ hΓ ((a.wk0 ⟨B, 0⟩).let₁ ((Γl.erase_left).cons (.left _))
+    (.pair (((Γl.erase.erase_left).cons (.right _)).cons (.left _)) .bv0 .bv1))
+  := by
+  rw [bind_pair_right _ _ _ _ _ he, bind_pair_left]
+  induction a, b using quotInd₂
+  apply sound; apply Wf.eqv.of_tm
+  rfl
+
+theorem Eqv.let_comm {A} {Γ Γl Γr : Ctx? α}
+  (hΓ : Γ.SSplit Γc Γr) (hΓc : Γc.SSplit Γl Γm) {ea eb : ε}
+  (a : Eqv R Γr A) (b : Eqv R Γm B) (c : Eqv R ((Γl.cons ⟨A, ⊤⟩).cons ⟨B, ⊤⟩) C)
+  [ha : a.HasEff ea] [hb : b.HasEff eb] (he : ea ⇌ eb)
+  : a.let₁ hΓ ((b.wk0 ⟨A, 0⟩).let₁ (hΓc.cons (.left _)) c)
+  = b.let₁ (hΓ.comm.s1_23_12_3 hΓc)
+    ((a.wk0 ⟨B, 0⟩).let₁ ((hΓ.comm.s1_23_12 hΓc).comm.cons (.left _))
+      (.let₁ ((((Ctx?.erase_right _).cons (.right _))).cons (.left _)) .bv1 (c.wk2 ⟨B, 0⟩)))
+  := by
+  rw [
+    let₂_beta_anti, <-let₁_bv0 (.let₁ _ .bv1 _), bind_pair_comm _ _ _ he, let₂_let₁, let₂_let₁,
+    let₂_beta
+  ]
+  induction a, b, c using quotInd₃
+  apply sound; apply Wf.eqv.of_tm
+  rfl
+
+theorem Eqv.let_comm_anti {A} {Γ Γl Γr : Ctx? α}
+  (hΓ : Γ.SSplit Γc Γr) (hΓc : Γc.SSplit Γl Γm) {ea eb : ε}
+  (a : Eqv R Γm A) (b : Eqv R Γr B) (c : Eqv R ((Γl.cons ⟨A, ⊤⟩).cons ⟨B, ⊤⟩) C)
+  [ha : a.HasEff ea] [hb : b.HasEff eb] (he : ea ⇌ eb)
+  : b.let₁ hΓ
+    ((a.wk0 ⟨B, 0⟩).let₁ (hΓc.cons (.left _))
+      (.let₁ ((((Ctx?.erase_right _).cons (.right _))).cons (.left _)) .bv1 (c.wk2 ⟨B, 0⟩)))
+  = a.let₁ (hΓ.comm.s1_23_12_3 hΓc)
+    ((b.wk0 ⟨A, 0⟩).let₁ ((hΓ.comm.s1_23_12 hΓc).comm.cons (.left _)) c)
+  := by
+  conv => rhs; rw [let_comm _ _ _ _ _ he]
+  induction a, b, c using quotInd₃
+  apply sound; apply Wf.eqv.of_tm
+  rfl
+
+def Eqv.reswap {A B} {Γ : Ctx? α} (a : Eqv R Γ (.tensor A B)) : Eqv R Γ (.tensor B A)
+  := .let₂ (Γ.erase_left) a (.pair ((Γ.erase.erase_left.cons (.right _)).cons (.left _)) .bv0 .bv1)
+
+theorem Eqv.reswap_let₁
+  {A B C} {Γ Γl Γr : Ctx? α} (hΓ : Γ.SSplit Γl Γr)
+    (a : Eqv R Γr A) (b : Eqv R (Γl.cons ⟨A, ⊤⟩) (.tensor B C))
+  : (a.let₁ hΓ b).reswap = a.let₁ hΓ b.reswap := by
+  rw [reswap, let₂_let₁]
+  induction a, b using quotInd₂
+  apply sound; apply Wf.eqv.of_tm
+  rfl
+
+theorem Eqv.reswap_let₂
+  {A B C D} {Γ Γl Γr : Ctx? α} (hΓ : Γ.SSplit Γl Γr)
+    (a : Eqv R Γr (.tensor A B)) (b : Eqv R ((Γl.cons ⟨A, ⊤⟩).cons ⟨B, ⊤⟩) (.tensor C D))
+  : (a.let₂ hΓ b).reswap = a.let₂ hΓ b.reswap := by
+  rw [reswap, let₂_let₂]
+  induction a, b using quotInd₂
+  apply sound; apply Wf.eqv.of_tm
+  rfl
+
+theorem Eqv.reswap_comm {A B} {Γ Γl Γr : Ctx? α}
+  (hΓ : Γ.SSplit Γl Γr) {ea eb : ε} (a : Eqv R Γl A) (b : Eqv R Γr B)
+  [ha : a.HasEff ea] [hb : b.HasEff eb] (he : ea ⇌ eb)
+  : (pair hΓ a b).reswap = (pair hΓ.comm b a) := by
+  rw [reswap, let₂_beta]
+  conv => rhs; rw [bind_pair_comm _ _ _ he.symm]
+  induction a, b using quotInd₂
+  apply sound; apply Wf.eqv.of_tm
+  rfl
+
+theorem Eqv.reswap_comm_left {A B} {Γ Γl Γr : Ctx? α}
+  (hΓ : Γ.SSplit Γl Γr) (a : Eqv R Γl A) (b : Eqv R Γr B) [ha : a.HasEff ⊥]
+  : (pair hΓ a b).reswap = (pair hΓ.comm b a)
+  := a.reswap_comm hΓ b (eb := ⊤) commutes_bot_left
+
+theorem Eqv.reswap_comm_right {A B} {Γ Γl Γr : Ctx? α}
+  (hΓ : Γ.SSplit Γl Γr) (a : Eqv R Γl A) (b : Eqv R Γr B) [hb : b.HasEff ⊥]
+  : (pair hΓ a b).reswap = (pair hΓ.comm b a)
+  := a.reswap_comm hΓ b (ea := ⊤) commutes_bot_right
+
+theorem Eqv.reswap_reswap {A B} {Γ : Ctx? α} (a : Eqv R Γ (.tensor A B)) : a.reswap.reswap = a := by
+  conv => lhs; rhs; rw [reswap]
+  rw [reswap_let₂, reswap_comm_left]
+  conv => rhs; rw [<-a.let₂_eta]
+  induction a using quotInd
+  apply sound; apply Wf.eqv.of_tm
+  simp only [Wf.let₂, Wf.pair, Wf.bv0, Wf.bv1]
+
+theorem Eqv.let₂_pair_right_wk0_wk0 {A B C D} {Γ Γc Γl Γm Γr : Ctx? α}
+  (hΓ : Γ.SSplit Γc Γr) (hΓc : Γc.SSplit Γl Γm)
+  (a : Eqv R Γr (.tensor A B)) (b : Eqv R ((Γl.cons ⟨A, ⊤⟩).cons ⟨B, ⊤⟩) C) (c : Eqv R Γm D)
+  : a.let₂ hΓ (.pair ((hΓc.cons (.left _)).cons (.left _)) b ((c.wk0 _).wk0 _))
+  = .pair (hΓ.comm.s1_23_12_3 hΓc) (.let₂ (hΓ.comm.s1_23_12 hΓc).comm a b) c
+  := by
+  conv => rhs; rw [bind_pair_left, let_let₂]
+  rw [bind_pair_left]
+  induction a, b, c using quotInd₃
+  apply sound; apply Wf.eqv.of_tm
+  simp only [
+    Wf.let₂, Wf.pair, Wf.bv0, Wf.bv1, Wf.let₁, Wf.wk0, Wf.wk1, ren_ren, <-Nat.liftWk_comp, ren,
+    Nat.liftWk_comp_succ
+  ]
+  rfl
+
+theorem Eqv.let₂_pair_right_bv2 {A B C} {Γ Γl Γr : Ctx? α}
+  (hΓ : (Γ.cons v).SSplit (Γl.cons ⟨X, ⊤⟩) (Γr.cons w))
+  (hΓc : (Γl.cons ⟨X, ⊤⟩).SSplit (Γl.cons ⟨X, 0⟩) (Γl.erase.cons ⟨X, ⊤⟩))
+  (a : Eqv R (Γr.cons w) (.tensor A B)) (b : Eqv R (((Γl.cons ⟨X, 0⟩).cons ⟨A, ⊤⟩).cons ⟨B, ⊤⟩) C)
+  : a.let₂ hΓ
+    (.pair ((hΓc.cons (.left _)).cons (.left _)) b .bv2)
+  = .pair (hΓ.comm.s1_23_12_3 hΓc)
+    (.let₂ (hΓ.comm.s1_23_12 hΓc).comm a b) .bv0
+  := let₂_pair_right_wk0_wk0 hΓ hΓc a b (.bv0)
