Refinery/Term/Extrinsic/Wf/Effect.lean
@@ -1,0 +1,167 @@
+import Refinery.Term.Extrinsic.Wf.Basic
+
+open HasQuant HasPQuant HasCommRel
+
+namespace Refinery
+
+namespace Term
+
+variable  {φ : Type u} {α : Type v} {ε : Type w} [S : Signature φ α ε] {R : DRWS φ α}
+
+abbrev Wf.HasEff (a : Wf R Γ A) (e : ε) := a.tm.HasEff e
+
+instance Wf.HasEff.top {a : Wf R Γ A} : a.HasEff ⊤
+  := Term.HasEff.top
+
+@[simp]
+instance Wf.HasEff.bv {Γ : Ctx? α} {A : Ty α} (e : ε) (i) (hv : Γ.At ⟨A, 1⟩ i)
+  : (Wf.bv (R := R) i hv).HasEff e
+  := Term.HasEff.bv i
+
+@[simp]
+instance Wf.HasEff.bv0 {Γ : Ctx? α} [hΓ : Γ.del] (e : ε)
+  : (Wf.bv0 (R := R) (Γ := Γ) (hΓ := hΓ) (q := q) (A := A)).HasEff e
+  := Term.HasEff.bv 0
+
+@[simp]
+instance Wf.HasEff.bv1 {Γ : Ctx? α} [hΓ : Γ.del] (e : ε) {v : Var? α} [hv : v.del]
+  : (Wf.bv1 (R := R) (Γ := Γ) (hΓ := hΓ) (v := v) (hv := hv) (q := q) (A := A)).HasEff e
+  := Term.HasEff.bv 1
+
+@[simp]
+instance Wf.HasEff.bv2 {Γ : Ctx? α} [hΓ : Γ.del] (e : ε) {l r : Var? α}
+  [hl : l.del] [hr : r.del]
+  : (
+      Wf.bv2 (R := R) (Γ := Γ) (hΓ := hΓ) (l := l) (hl := hl) (r := r) (hr := hr) (q := q) (A := A)
+    ).HasEff e
+  := Term.HasEff.bv 2
+
+@[simp]
+instance Wf.HasEff.bv3 {Γ : Ctx? α} [hΓ : Γ.del] (e : ε) {l m r : Var? α}
+  [hl : l.del] [hm : m.del] [hr : r.del]
+  : (
+      Wf.bv3 (R := R) (Γ := Γ) (hΓ := hΓ)
+        (l := l) (hl := hl) (m := m) (hm := hm) (r := r) (hr := hr)
+        (q := q) (A := A)
+    ).HasEff e
+  := Term.HasEff.bv 3
+
+theorem Wf.HasEff.pair {Γ Γl Γr : Ctx? α} (hΓ : Γ.SSplit Γl Γr) {A B : Ty α}
+  {a : Wf R Γl A} {b : Wf R Γr B} {e : ε}
+  (ha : a.HasEff e) (hb : b.HasEff e) : (pair hΓ a b).HasEff e
+  := Term.HasEff.pair ha hb
+
+instance Wf.HasEff.instPair {Γ Γl Γr : Ctx? α} (hΓ : Γ.SSplit Γl Γr) {A B : Ty α}
+  (a : Wf R Γl A) (b : Wf R Γr B) (e : ε)
+  [ha : a.HasEff e] [hb : b.HasEff e] : (Wf.pair hΓ a b).HasEff e
+  := ha.pair hΓ hb
+
+theorem Wf.HasEff.let₁ {Γ Γl Γr : Ctx? α} (hΓ : Γ.SSplit Γl Γr) {A B : Ty α}
+  {a : Wf R Γr A} {b : Wf R (Γl.cons ⟨A, ⊤⟩) B} {e : ε}
+  (ha : a.HasEff e) (hb : b.HasEff e) : (a.let₁ hΓ b).HasEff e
+  := Term.HasEff.let₁ ha hb
+
+instance Wf.HasEff.instLet₁ {Γ Γl Γr : Ctx? α} (hΓ : Γ.SSplit Γl Γr) {A B : Ty α}
+  (a : Wf R Γr A) (b : Wf R (Γl.cons ⟨A, ⊤⟩) B) (e : ε)
+  [ha : a.HasEff e] [hb : b.HasEff e] : (Wf.let₁ hΓ a b).HasEff e
+  := ha.let₁ hΓ hb
+
+theorem Wf.HasEff.let₂ {Γ Γl Γr : Ctx? α} (hΓ : Γ.SSplit Γl Γr) {A B C : Ty α}
+  {a : Wf R Γr (A.tensor B)} {b : Wf R ((Γl.cons ⟨A, ⊤⟩).cons ⟨B, ⊤⟩) C} {e : ε}
+  (ha : a.HasEff e) (hb : b.HasEff e) : (a.let₂ hΓ b).HasEff e
+  := Term.HasEff.let₂ ha hb
+
+instance Wf.HasEff.instLet₂ {Γ Γl Γr : Ctx? α} (hΓ : Γ.SSplit Γl Γr) {A B C : Ty α}
+  (a : Wf R Γr (A.tensor B)) (b : Wf R ((Γl.cons ⟨A, ⊤⟩).cons ⟨B, ⊤⟩) C) (e : ε)
+  [ha : a.HasEff e] [hb : b.HasEff e] : (Wf.let₂ hΓ a b).HasEff e
+  := ha.let₂ hΓ hb
+
+theorem Wf.HasEff.case {Γ Γl Γr : Ctx? α} (hΓ : Γ.SSplit Γl Γr) {A B C : Ty α}
+  {a : Wf R Γr (A.coprod B)} {b : Wf R (Γl.cons ⟨A, ⊤⟩) C}
+  {c : Wf R (Γl.cons ⟨B, ⊤⟩) C} {e : ε}
+  (ha : a.HasEff e) (hb : b.HasEff e) (hc : c.HasEff e)
+  : (a.case hΓ b c).HasEff e
+  := Term.HasEff.case ha hb hc
+
+instance Wf.HasEff.instCase {Γ Γl Γr : Ctx? α} (hΓ : Γ.SSplit Γl Γr) {A B C : Ty α}
+  (a : Wf R Γr (A.coprod B)) (b : Wf R (Γl.cons ⟨A, ⊤⟩) C)
+  (c : Wf R (Γl.cons ⟨B, ⊤⟩) C) (e : ε)
+  [ha : a.HasEff e] [hb : b.HasEff e] [hc : c.HasEff e] : (Wf.case hΓ a b c).HasEff e
+  := ha.case hΓ hb hc
+
+theorem Wf.HasEff.iter {Γ Γl Γr : Ctx? α} (hΓ : Γ.SSplit Γl Γr) {A B : Ty α}
+  {a : Wf R Γr A} {b : Wf R (Γl.cons ⟨A, ⊤⟩) (B.coprod A)} {e : ε}
+  (he : e ∈ S.iterative) (hc : Γl.copy) (hd : Γl.del)
+  (ha : a.HasEff e) (hb : b.HasEff e) : (a.iter (hc := hc) (hd := hd) hΓ b).HasEff e
+  := Term.HasEff.iter he ha hb
+
+instance Wf.HasEff.instIter {Γ Γl Γr : Ctx? α} (hΓ : Γ.SSplit Γl Γr) {A B : Ty α}
+  (a : Wf R Γr A) (b : Wf R (Γl.cons ⟨A, ⊤⟩) (B.coprod A)) (e : ε)
+  (he : e ∈ S.iterative) (hc : Γl.copy) (hd : Γl.del)
+  [ha : a.HasEff e] [hb : b.HasEff e] : (Wf.iter hΓ a b).HasEff e
+  := ha.iter hΓ he hc hd hb
+
+inductive Eqv.HasEff {Γ : Ctx? α} {A : Ty α} : Eqv R Γ A → ε → Prop
+  | mk {a : Wf R Γ A} (ha : a.HasEff e) : Eqv.HasEff e⟦a⟧ e
+
+attribute [class] Eqv.HasEff
+
+attribute [instance] Eqv.HasEff.mk
+
+instance Eqv.HasEff.top {a : Eqv R Γ A} : a.HasEff ⊤
+  := by induction a using quotInd; constructor; infer_instance
+
+instance Eqv.HasEff.bv {Γ : Ctx? α} {A : Ty α} (e : ε) (i) (hv : Γ.At ⟨A, 1⟩ i)
+  : Eqv.HasEff (Eqv.bv (R := R) i hv) e := .mk (.bv e i hv)
+
+instance Eqv.HasEff.bv0 {Γ : Ctx? α} [hΓ : Γ.del] (e : ε)
+  : Eqv.HasEff (Eqv.bv0 (R := R) (Γ := Γ) (hΓ := hΓ) (q := q) (A := A)) e
+  := .mk (.bv0 e)
+
+instance Eqv.HasEff.bv1 {Γ : Ctx? α} [hΓ : Γ.del] (e : ε) {v : Var? α} [hv : v.del]
+  : Eqv.HasEff (Eqv.bv1 (R := R) (Γ := Γ) (hΓ := hΓ) (v := v) (hv := hv) (q := q) (A := A)) e
+  := .mk (.bv1 e)
+
+instance Eqv.HasEff.bv2 {Γ : Ctx? α} [hΓ : Γ.del] (e : ε) {l r : Var? α}
+  [hl : l.del] [hr : r.del]
+  : Eqv.HasEff (
+    Eqv.bv2 (R := R) (Γ := Γ) (hΓ := hΓ) (l := l) (hl := hl) (r := r) (hr := hr) (q := q) (A := A)
+  ) e
+  := .mk (.bv2 e)
+
+instance Eqv.HasEff.bv3 {Γ : Ctx? α} [hΓ : Γ.del] (e : ε) {l m r : Var? α}
+  [hl : l.del] [hm : m.del] [hr : r.del]
+  : Eqv.HasEff (
+    Eqv.bv3 (R := R) (Γ := Γ) (hΓ := hΓ)
+      (l := l) (hl := hl) (m := m) (hm := hm) (r := r) (hr := hr)
+      (q := q) (A := A)
+  ) e
+  := .mk (.bv3 e)
+
+instance Eqv.HasEff.pair {Γ Γl Γr : Ctx? α} (hΓ : Γ.SSplit Γl Γr) {A B : Ty α}
+  {a : Eqv R Γl A} {b : Eqv R Γr B} (e : ε)
+  (ha : a.HasEff e) (hb : b.HasEff e) : Eqv.HasEff (Eqv.pair hΓ a b) e
+  := by cases ha; cases hb; constructor; infer_instance
+
+instance Eqv.HasEff.let₁ {Γ Γl Γr : Ctx? α} (hΓ : Γ.SSplit Γl Γr) {A B : Ty α}
+  {a : Eqv R Γr A} {b : Eqv R (Γl.cons ⟨A, ⊤⟩) B} (e : ε)
+  (ha : a.HasEff e) (hb : b.HasEff e) : Eqv.HasEff (Eqv.let₁ hΓ a b) e
+  := by cases ha; cases hb; constructor; infer_instance
+
+instance Eqv.HasEff.let₂ {Γ Γl Γr : Ctx? α} (hΓ : Γ.SSplit Γl Γr) {A B C : Ty α}
+  {a : Eqv R Γr (A.tensor B)} {b : Eqv R ((Γl.cons ⟨A, ⊤⟩).cons ⟨B, ⊤⟩) C} (e : ε)
+  (ha : a.HasEff e) (hb : b.HasEff e) : Eqv.HasEff (Eqv.let₂ hΓ a b) e
+  := by cases ha; cases hb; constructor; infer_instance
+
+instance Eqv.HasEff.case {Γ Γl Γr : Ctx? α} (hΓ : Γ.SSplit Γl Γr) {A B C : Ty α}
+  {a : Eqv R Γr (A.coprod B)} {b : Eqv R (Γl.cons ⟨A, ⊤⟩) C}
+  {c : Eqv R (Γl.cons ⟨B, ⊤⟩) C} (e : ε)
+  (ha : a.HasEff e) (hb : b.HasEff e) (hc : c.HasEff e)
+  : Eqv.HasEff (Eqv.case hΓ a b c) e
+  := by cases ha; cases hb; cases hc; constructor; infer_instance
+
+instance Eqv.HasEff.iter {Γ Γl Γr : Ctx? α} (hΓ : Γ.SSplit Γl Γr) {A B : Ty α}
+  {a : Eqv R Γr A} {b : Eqv R (Γl.cons ⟨A, ⊤⟩) (B.coprod A)} (e : ε)
+  (he : e ∈ S.iterative) (hc : Γl.copy) (hd : Γl.del)
+  (ha : a.HasEff e) (hb : b.HasEff e) : Eqv.HasEff (Eqv.iter hΓ a b) e
+  := by cases ha; cases hb; constructor; apply Wf.HasEff.iter <;> assumption
