Refinery/Term/Extrinsic/Wf/PreBeta.lean
@@ -1,5 +1,6 @@
 import Refinery.Term.Extrinsic.Refinement.Wk.Relation
 import Refinery.Term.Extrinsic.Wf.Wk
+import Refinery.Term.Extrinsic.Wf.Effect
 import Refinery.Term.Extrinsic.FreeVar
 
 open HasQuant HasPQuant HasCommRel
@@ -15,7 +16,7 @@ variable  {φ : Type u} {α : Type v} {ε : Type w} [S : Signature φ α ε]
 theorem Wf.pre_beta_pos  {Γ Γl Γr : Ctx? α} {A : Ty α}
   (hΓ : Γ.SSplit Γl Γr) (a : Wf R Γr A) (q : Quant) (hq : q ⊓ quant A ≤ quant Γr)
   (b : Wf R (Γl.cons ⟨A, q⟩) B)
-  {el er} [ha : HasEff el a.tm] [hb : HasEff er b.tm] (he : el ⇀ er)
+  {el er} [ha : a.HasEff el] [hb : b.HasEff er] (he : el ⇀ er)
   (heq : q ⊓ quant A ≤ (pquant el).pos)
   : a.let₁ hΓ (b.pwk ((Ctx?.PWk.refl Γl).cons (by simp))) ≤ b.subst (SubstDS.subst0 hΓ a.deriv q hq)
     := by
@@ -26,7 +27,7 @@ theorem Wf.pre_beta_pos  {Γ Γl Γr : Ctx? α} {A : Ty α}
 theorem Wf.pre_beta_neg {Γ Γl Γr : Ctx? α} {A : Ty α}
     (hΓ : Γ.SSplit Γl Γr) (a : Wf R Γr A) (q : Quant) (hq : q ⊓ quant A ≤ quant Γr)
     (b : Wf R (Γl.cons ⟨A, q⟩) B)
-    {el er} [ha : HasEff el a.tm] [hb : HasEff er b.tm] (he : el ↽ er)
+    {el er} [ha : a.HasEff el] [hb : b.HasEff er] (he : el ↽ er)
     (heq : q ⊓ quant A ≤ (pquant el).neg)
     : a.let₁ hΓ (b.pwk ((Ctx?.PWk.refl Γl).cons (by simp)))
     ≥ b.subst (SubstDS.subst0 hΓ a.deriv q hq)
@@ -38,16 +39,16 @@ theorem Wf.pre_beta_neg {Γ Γl Γr : Ctx? α} {A : Ty α}
 theorem Wf.pre_beta {Γ Γl Γr : Ctx? α} {A : Ty α}
     (hΓ : Γ.SSplit Γl Γr) (a : Wf R Γr A) (q : Quant) (hq : q ⊓ quant A ≤ quant Γr)
     (b : Wf R (Γl.cons ⟨A, q⟩) B)
-    {el er} [ha : HasEff el a.tm] [hb : HasEff er b.tm] (he : el ⇌ er)
+    {el er} [ha : a.HasEff el] [hb : b.HasEff er] (he : el ⇌ er)
     (heq : q ⊓ quant A ≤ (pquant el))
     : a.let₁ hΓ (b.pwk ((Ctx?.PWk.refl Γl).cons (by simp)))
     ≈ b.subst (SubstDS.subst0 hΓ a.deriv q hq)
     := ⟨pre_beta_pos hΓ a q hq b he.left heq.left, pre_beta_neg hΓ a q hq b he.right heq.right⟩
 
-theorem Wf.pre_beta_pureIn {Γ Γl Γr : Ctx? α} {A : Ty α}
+theorem Wf.pre_beta_pureIn {B} {Γ Γl Γr : Ctx? α} {A : Ty α}
     (hΓ : Γ.SSplit Γl Γr) (a : Wf R Γr A) (q : Quant) (hq : q ⊓ quant A ≤ quant Γr)
     (b : Wf R (Γl.cons ⟨A, q⟩) B)
-    [ha : HasEff ⊥ a.tm]
+    [ha : a.HasEff ⊥]
     : a.let₁ hΓ (b.pwk ((Ctx?.PWk.refl Γl).cons (by simp)))
     ≈ b.subst (SubstDS.subst0 hΓ a.deriv q hq)
     := pre_beta hΓ a q hq b (commutes_bot_left (r := ⊤)) (by simp [OrderedPQuant.pquant_bot])
@@ -55,7 +56,7 @@ theorem Wf.pre_beta_pureIn {Γ Γl Γr : Ctx? α} {A : Ty α}
 theorem Wf.pre_beta_pureLin {Γ Γl Γr : Ctx? α} {A : Ty α}
     (hΓ : Γ.SSplit Γl Γr) (a : Wf R Γr A)
     (b : Wf R (Γl.cons ⟨A, 1⟩) B)
-    [ha : HasEff ⊥ a.tm]
+    [ha : a.HasEff ⊥]
     : a.let₁ hΓ (b.pwk ((Ctx?.PWk.refl Γl).cons (by simp)))
     ≈ b.subst (SubstDS.subst0 hΓ a.deriv 1 bot_le)
     := pre_beta_pureIn hΓ a 1 bot_le b
@@ -63,7 +64,7 @@ theorem Wf.pre_beta_pureLin {Γ Γl Γr : Ctx? α} {A : Ty α}
 theorem Wf.pre_beta_pureLout {Γ Γl Γr : Ctx? α} {A : Ty α}
     (hΓ : Γ.SSplit Γl Γr) (a : Wf R Γr A)
     (b : Wf R (Γl.cons ⟨A, 1⟩) B)
-    [hb : HasEff ⊥ b.tm]
+    [hb : b.HasEff ⊥]
     : a.let₁ hΓ (b.pwk ((Ctx?.PWk.refl Γl).cons (by simp)))
     ≈ b.subst (SubstDS.subst0 hΓ a.deriv 1 bot_le)
     := pre_beta hΓ a 1 bot_le b (commutes_bot_right (l := ⊤)) bot_le
@@ -71,11 +72,11 @@ theorem Wf.pre_beta_pureLout {Γ Γl Γr : Ctx? α} {A : Ty α}
 theorem Wf.let₁_eta_pwk {Γ Γl Γr : Ctx? α}
   {A : Ty α} (a : Wf R Γr A) (hΓ : Γ.SSplit Γl Γr) [hΓl : Γl.del]
   : a.let₁ hΓ .bv0 ≈ a.pwk (hΓ.pwk_left_del) := by
-  apply (Wf.pre_beta_pureLout hΓ a .bv0 (hb := by simp [bv0])).coh <;> rfl
+  apply (Wf.pre_beta_pureLout hΓ a .bv0 (hb := by simp)).coh <;> rfl
 
 theorem Wf.let₁_eta' {Γ : Ctx? α} {A : Ty α}
   (a : Wf R Γ A) (hΓ : Γ.SSplit Γl Γ) [hΓl : Γl.del] : a.let₁ hΓ .bv0 ≈ a := by
-  apply (Wf.pre_beta_pureLout hΓ a .bv0 (hb := by simp [bv0])).coh <;> rfl
+  apply (Wf.pre_beta_pureLout hΓ a .bv0 (hb := by simp)).coh <;> rfl
 
 theorem Wf.let₁_eta {Γ : Ctx? α} {A : Ty α} (a : Wf R Γ A) : a.let₁ Γ.erase_left .bv0 ≈ a
 := a.let₁_eta' _
@@ -98,7 +99,7 @@ theorem Wf.let₁_bv0 {Γ : Ctx? α} {A B : Ty α} (a : Wf R (Γ.cons ⟨A, ⊤�
   := by
     apply (Wf.pre_beta_pureIn
       (Γ.erase_right.cons (.right ⟨A, ⊤⟩)) .bv0 (quant A) (by simp; simp [quant])
-        ((a.pwk ((Ctx?.PWk.refl _).cons (.wk (by simp)))).wk1 _) (ha := by simp [bv0])).coh
+        ((a.pwk ((Ctx?.PWk.refl _).cons (.wk (by simp)))).wk1 _) (ha := by simp)).coh
     · rfl
     · cases a;
       simp only [subst, EQuant.coe_top, pwk, wk1, ← subst_renIn]
@@ -136,12 +137,14 @@ theorem Eqv.let₁_unit_anti [R.UWkCongr] {Γ : Ctx? α} {A : Ty α} (a : Eqv R 
 theorem Wf.bind_pwk_inl {Γ Γl Γr : Ctx? α}
   {A : Ty α} (a : Wf R Γr A) (hΓ : Γ.SSplit Γl Γr) [hΓl : Γl.del]
   : a.let₁ hΓ (.inl A B .bv0) ≈ (a.pwk (hΓ.pwk_left_del)).inl A B := by
-  apply (Wf.pre_beta_pureLout hΓ a (.inl A B .bv0) (hb := by simp [inl, bv0])).coh <;> rfl
+  apply (Wf.pre_beta_pureLout hΓ a (.inl A B .bv0) (hb := by simp [Wf.HasEff, inl, bv0])).coh
+  <;> rfl
 
 theorem Wf.bind_inl' {Γ : Ctx? α} {A : Ty α}
   (a : Wf R Γ A) (hΓ : Γ.SSplit Γl Γ) [hΓl : Γl.del]
   : a.let₁ hΓ (.inl A B .bv0) ≈ a.inl A B := by
-  apply (Wf.pre_beta_pureLout hΓ a (.inl A B .bv0) (hb := by simp [inl, bv0])).coh <;> rfl
+  apply (Wf.pre_beta_pureLout hΓ a (.inl A B .bv0) (hb := by simp [Wf.HasEff, inl, bv0])).coh
+  <;> rfl
 
 theorem Wf.bind_inl {Γ : Ctx? α} {A : Ty α} (a : Wf R Γ A)
   : a.let₁ Γ.erase_left (.inl A B .bv0) ≈ a.inl A B
@@ -164,12 +167,14 @@ theorem Eqv.bind_inl {Γ : Ctx? α} {A : Ty α} (a : Eqv R Γ A)
 theorem Wf.bind_pwk_inr {Γ Γl Γr : Ctx? α}
   {A : Ty α} (a : Wf R Γr A) (hΓ : Γ.SSplit Γl Γr) [hΓl : Γl.del]
   : a.let₁ hΓ (.inr B A .bv0) ≈ (a.pwk (hΓ.pwk_left_del)).inr B A := by
-  apply (Wf.pre_beta_pureLout hΓ a (.inr B A .bv0) (hb := by simp [inr, bv0])).coh <;> rfl
+  apply (Wf.pre_beta_pureLout hΓ a (.inr B A .bv0) (hb := by simp [Wf.HasEff, inr, bv0])).coh
+  <;> rfl
 
 theorem Wf.bind_inr' {Γ : Ctx? α} {A : Ty α}
   (a : Wf R Γ A) (hΓ : Γ.SSplit Γl Γ) [hΓl : Γl.del]
   : a.let₁ hΓ (.inr B A .bv0) ≈ a.inr B A := by
-  apply (Wf.pre_beta_pureLout hΓ a (.inr B A .bv0) (hb := by simp [inr, bv0])).coh <;> rfl
+  apply (Wf.pre_beta_pureLout hΓ a (.inr B A .bv0) (hb := by simp [Wf.HasEff, inr, bv0])).coh
+  <;> rfl
 
 theorem Wf.bind_inr {Γ : Ctx? α} {A : Ty α} (a : Wf R Γ A)
   : a.let₁ Γ.erase_left (.inr B A .bv0) ≈ a.inr B A
@@ -192,12 +197,14 @@ theorem Eqv.bind_inr {Γ : Ctx? α} {A : Ty α} (a : Eqv R Γ A)
 theorem Wf.bind_pwk_abort {Γ Γl Γr : Ctx? α}
   {A : Ty α} (a : Wf R Γr .empty) (hΓ : Γ.SSplit Γl Γr) [hΓl : Γl.del]
   : a.let₁ hΓ (.abort A .bv0) ≈ (a.pwk (hΓ.pwk_left_del)).abort A := by
-  apply (Wf.pre_beta_pureLout hΓ a (.abort A .bv0) (hb := by simp [abort, bv0])).coh <;> rfl
+  apply (Wf.pre_beta_pureLout hΓ a (.abort A .bv0) (hb := by simp [Wf.HasEff, abort, bv0])).coh
+  <;> rfl
 
 theorem Wf.bind_abort' {Γ : Ctx? α} {A : Ty α}
   (a : Wf R Γ .empty) (hΓ : Γ.SSplit Γl Γ) [hΓl : Γl.del]
   : a.let₁ hΓ (.abort A .bv0) ≈ a.abort A := by
-  apply (Wf.pre_beta_pureLout hΓ a (.abort A .bv0) (hb := by simp [abort, bv0])).coh <;> rfl
+  apply (Wf.pre_beta_pureLout hΓ a (.abort A .bv0) (hb := by simp [Wf.HasEff, abort, bv0])).coh
+  <;> rfl
 
 theorem Wf.bind_abort {Γ : Ctx? α} {A : Ty α} (a : Wf R Γ .empty)
   : a.let₁ Γ.erase_left (.abort A .bv0) ≈ a.abort A
